RegexCorrectness/Data/String.lean
@@ -41,6 +41,10 @@ theorem ext {it₁ it₂ : Iterator} (hs : it₁.s = it₂.s) (hi : it₁.i = it
 theorem ext_iff {it₁ it₂ : Iterator} : it₁ = it₂ ↔ it₁.s = it₂.s ∧ it₁.i = it₂.i :=
   ⟨fun h => ⟨h ▸ rfl, h ▸ rfl⟩, fun ⟨hs, hi⟩ => ext hs hi⟩
 
+theorem hasNext_of_not_atEnd {it : Iterator} (h : ¬it.atEnd) : it.hasNext := by
+  simp [hasNext, atEnd] at *
+  exact h
+
 end String.Iterator
 
 namespace String.Iterator.Valid
